theories/Misc/Head.v
@@ -114,11 +114,11 @@ Proof.
     rewrite <- ctree_eta; symmetry; assumption.
 Qed.
 
-Lemma trans_head_obs_void : forall (t u : ctree E B X) (e : E void),
-    ~ trans (obs_void e) t u.
+Lemma trans_head_die : forall {Y} (t u : ctree E B X) (e : E Y) (empty : forall (y : Y), False),
+    ~ trans (die e empty) t u.
 Proof.
   intros * TR.
-  remember (obs_void e) as ob.
+  remember (die e empty) as ob.
   induction TR; try now inv Heqob.
 Qed.
 
@@ -184,14 +184,18 @@ Lemma trans_head : forall (t u : ctree E B X) l,
         trans (val (AStep u')) (head t : ctree F C _) Stuck /\ u' ≅ u
     | obs e v => exists (k : _ -> ctree E B X),
         trans (val (AVis e k)) (head t : ctree F C _) Stuck /\ u ≅ k v
-    | obs_void e => False
+    | die e empty => False
     | val v => trans (val (@ARet E B _ v)) (head t : ctree F C _) Stuck /\ u ≅ Stuck
     end.
 Proof.
   intros *; destruct l.
   apply trans_head_tau.
   apply trans_head_obs.
-  apply trans_head_obs_void.
+  { intros TRANS.
+    eapply (@trans_head_die _ t u e empty).
+    Set Printing Implicit.
+    apply TRANS.
+  }
   intros A.
   pose proof (trans_val_invT A) as <-; apply trans_head_ret; assumption.
 Qed.
